Try out Dblib

theories/Substitution.v
@@ -4,7 +4,10 @@ From MailboxTypes Require Export Environment.
 From MailboxTypes Require Export Syntax.
 From MailboxTypes Require Import Util.
 From MailboxTypes Require Import TypingRules.
+From MailboxTypes Require Import Dblib.DeBruijn.
+From MailboxTypes Require Import Dblib.DblibTactics.
 
+From Stdlib Require Import Lia.
 
 (** We assume functional extensionality in order to proof statements about substitutions. *)
 From Stdlib Require Import FunctionalExtensionality.
@@ -17,7 +20,378 @@ Section subs_def.
   Context `{M : IMessage Message}.
   Context `{D : IDefinitionName DefinitionName}.
 
-  (**
+
+  Instance Var_Value : Var Value :=
+  {
+    var := ValueVar
+  }.
+
+  Definition traverse_Value (f : nat -> nat -> Value) l v :=
+    match v with
+    | ValueVar x => f l x
+    | v' => v'
+    end.
+
+  Fixpoint traverse_Term (f : nat -> nat -> Value) l t :=
+    match t with
+    | TValue v => TValue (traverse_Value f l v)
+    | TLet t1 t2  => TLet (traverse_Term f l t1) (traverse_Term f (l+1) t2)
+    | TApp def v => TApp def (traverse_Value f l v)
+    | TSpawn t1 => TSpawn (traverse_Term f l t1)
+    | TNew => TNew
+    | TSend v1 m v2 => TSend (traverse_Value f l v1) m (traverse_Value f l v2)
+    | TGuard v e guards => TGuard (traverse_Value f l v) e (map (traverse_Guard f l) guards)
+    end
+  with traverse_Guard (f : nat -> nat -> Value) l g :=
+match g with
+    | GFail => GFail
+    | GFree t1 => GFree (traverse_Term f l t1)
+    (* Assumption: we only receive one value in the message *)
+    | GReceive m t1 => GReceive m (traverse_Term f (l+2) t1)
+    end.
+
+  Instance Traverse_Value_Value : Traverse Value Value :=
+  {
+    traverse := traverse_Value
+  }.
+
+  Instance Traverse_Value_Term : Traverse Value Term :=
+  {
+    traverse := traverse_Term
+  }.
+
+  Instance Traverse_Value_Guard : Traverse Value Guard :=
+  {
+    traverse := traverse_Guard
+  }.
+
+  Instance TraverseVarInjective_Value : @TraverseVarInjective Value _ Value _.
+  Proof.
+    constructor; prove_traverse_var_injective.
+  Qed.
+
+  Lemma traverse_Guards_injective : forall (l1 l2 : list Guard) f n,
+    map (traverse_Guard (fun l x : nat => ValueVar (f l x)) n) l1 =
+    map (traverse_Guard (fun l x : nat => ValueVar (f l x)) n) l2 ->
+    (forall x1 x2 l : nat, f l x1 = f l x2 -> x1 = x2) ->
+    (forall f : nat -> nat -> nat,
+    (forall x1 x2 l : nat, f l x1 = f l x2 -> x1 = x2) ->
+    forall (t1 t2 : Guard) (l : nat),
+    traverse_var f l t1 = traverse_var f l t2 -> t1 = t2) ->
+    l1 = l2.
+  Proof.
+    induction l1, l2; intros * MapInj ? TravInj; try (reflexivity || discriminate).
+    injection MapInj; intros ? Inj.
+    apply TravInj in Inj; subst; try (f_equal; eapply IHl1); eassumption.
+  Qed.
+
+  Ltac prove_traverse_var_injective :=
+    let t1 := fresh "t1" in
+    intros ? ? t1; induction t1;
+    let t2 := fresh "t2" in
+    intro t2; destruct t2; simpl;
+    let h := fresh "h" in
+    intros ? h; inversion h;
+    f_equal;
+    eauto using @traverse_var_injective with typeclass_instances.
+    (* The lemma [traverse_var_injective] can be useful if the [traverse]
+      function at hand calls another [traverse] function which has already
+      been proved injective. *)
+
+  Lemma traverse_Value_injective :
+    forall f : nat -> nat -> nat,
+    (forall x1 x2 l : nat, f l x1 = f l x2 -> x1 = x2) ->
+    forall (v1 v2 : Value) (l : nat),
+    traverse_var f l v1 = traverse_var f l v2 -> v1 = v2.
+  Proof.
+    intros until v1. induction v1, v2; intros n InjV;
+    inversion InjV; f_equal; try easy;
+    eapply H; eassumption.
+  Qed.
+
+  Lemma traverse_Term_injective :
+    forall (f : nat -> nat -> nat)
+    (inj : (forall x1 x2 l : nat, f l x1 = f l x2 -> x1 = x2))
+    (t1 t2 : Term) (l : nat),
+    traverse_var f l t1 = traverse_var f l t2 -> t1 = t2.
+  Proof.
+    intros until t1.
+    induction t1 using @Term_ind3
+      with (PG := fun g1 => forall (g2 : Guard) (l : nat),
+        traverse_var f l g1 = traverse_var f l g2 -> g1 = g2);
+    intro t2; destruct t2; simpl; intros n Inj; inversion Inj; f_equal;
+    try (eapply traverse_Value_injective; eassumption);
+    try ((eapply IHt1 || eapply IHt1_1 || eapply IHt1_2); eassumption).
+    subst; generalize dependent l.
+    induction gs; simpl in *; intros * Eql mTrav.
+    - symmetry in mTrav; now apply map_eq_nil in mTrav.
+    - inversion H; subst.
+      symmetry in mTrav; apply map_eq_cons in mTrav.
+      destruct mTrav as [g' [l' [Eq [Eq2 Eq3]]]]; subst.
+      erewrite H3 with (g2 := g').
+      * f_equal; apply IHgs; eauto.
+        f_equal; eauto.
+      * eauto.
+  Qed.
+
+  Instance TraverseVarInjective_Term : @TraverseVarInjective Value _ Term _.
+  Proof. constructor; apply traverse_Term_injective. Qed.
+
+  Lemma traverse_Value_functorial : forall f g (v : Value) l,
+    traverse g l (traverse f l v) = traverse (fun l x => traverse g l (f l x)) l v.
+  Proof.
+    prove_traverse_functorial.
+  Qed.
+
+  Lemma traverse_Term_functorial : forall f g (t : Term) l,
+    traverse g l (traverse f l t) = traverse (fun l x => traverse g l (f l x)) l t.
+  Proof.
+    intros until t.
+    induction t using @Term_ind3
+      with (PG := fun g1 => forall (l : nat),
+      traverse g l (traverse f l g1) = traverse (fun l x => traverse g l (f l x)) l g1);
+    intros l; simpl; f_equal; try (apply traverse_Value_functorial);
+    try (apply IHt || apply IHt1 || apply IHt2).
+    induction gs; simpl in *.
+    - reflexivity.
+    - inversion H as [| ? ? Eq]. subst. rewrite IHgs.
+      * now rewrite Eq.
+      * assumption.
+  Qed.
+
+  Instance TraverseFunctorial_Value : @TraverseFunctorial Value _ Value _.
+  Proof. constructor; apply traverse_Value_functorial. Qed.
+
+  Instance TraverseFunctorial_Term : @TraverseFunctorial Value _ Term _.
+  Proof. constructor; apply traverse_Term_functorial. Qed.
+
+  Instance TraverseIdentifiesVar_Value : TraverseIdentifiesVar.
+  Proof. constructor; prove_traverse_identifies_var. Qed.
+
+  Lemma traverse_Value_relative :
+    forall (f g : nat -> nat -> Value) (p : nat) (v : Value) (m l : nat),
+    (forall l' x : nat, f (l' + p) x = g l' x) ->
+    m = l + p -> traverse f m v = traverse g l v.
+  Proof.
+    intros * Eq natEq.
+    destruct v; simpl; try easy.
+    rewrite natEq; apply Eq.
+  Qed.
+
+  Lemma traverse_Term_relative :
+    forall (f g : nat -> nat -> Value) (p : nat) (t : Term) (m l : nat),
+    (forall l' x : nat, f (l' + p) x = g l' x) ->
+    m = l + p -> traverse f m t = traverse g l t.
+  Proof.
+    intros until t.
+    induction t using @Term_ind3
+      with (PG := fun g1 => forall (m l : nat),
+      (forall l' x : nat, f (l' + p) x = g l' x) ->
+      m = l + p -> traverse f m g1 = traverse g l g1);
+    intros * Eq natEq; simpl; f_equal;
+    try (eapply traverse_Value_relative; eassumption);
+    try (apply IHt1 || apply IHt2 || apply IHt); try (assumption || lia).
+    induction gs.
+    - reflexivity.
+    - inversion H as [| ? ? EqInd]; subst; simpl in *.
+      erewrite EqInd.
+      + f_equal; apply IHgs; assumption.
+      + assumption.
+      + lia.
+  Qed.
+
+  Instance TraverseRelative_Value : @TraverseRelative Value Value _.
+  Proof. constructor; apply traverse_Value_relative. Qed.
+
+  Instance TraverseRelative_Term : @TraverseRelative Value Term _.
+  Proof. constructor; apply traverse_Term_relative. Qed.
+
+  Lemma traverse_Value_identity:
+    forall f,
+    (forall l x, f l x = var x) ->
+    forall (v : Value) l,
+    traverse f l v = v.
+  Proof.
+    intros; destruct v; simpl; try reflexivity; now rewrite H.
+  Qed.
+
+  Lemma traverse_Term_identity:
+    forall f,
+    (forall l x, f l x = var x) ->
+    forall (t : Term) l,
+    traverse f l t = t.
+  Proof.
+    intros until t.
+    induction t as [| | | | | | ? ? ? Fs | | | ] using @Term_ind3
+      with (PG := fun g1 => forall (l : nat), traverse f l g1 = g1);
+    intros; simpl; f_equal;
+    try (eapply traverse_Value_identity; eassumption);
+    try (apply IHt1 || apply IHt2 || apply IHt); try (assumption || lia).
+    induction gs.
+    - reflexivity.
+    - simpl in *. inversion Fs as [| ? ? EqInd]; subst.
+      rewrite EqInd; f_equal; apply IHgs; assumption.
+  Qed.
+
+  Instance TraverseVarIsIdentity_Value : @TraverseVarIsIdentity Value _ Value _.
+  Proof. constructor; apply traverse_Value_identity. Qed.
+
+  Instance TraverseVarIsIdentity_Term : @TraverseVarIsIdentity Value _ Term _.
+  Proof. constructor; apply traverse_Term_identity. Qed.
+
+  (* First argument: Value *)
+  (* Second argument: Variable *)
+  (* Third argument: Term *)
+  Type @subst Value Term.
+
+
+  Lemma EmptyEnv_app_cons : forall env1 env2 T, ~ EmptyEnv (env1 ++ Some T :: env2).
+  Proof.
+    induction env1; intros.
+    - intros E; inversion E; subst; discriminate.
+    - destruct a; intros E; inversion E; subst.
+      + discriminate.
+      + now apply IHenv1 in H2.
+  Qed.
+
+  Lemma SingletonEnv_app_cons : forall env1 env2 T,
+    SingletonEnv (env1 ++ Some T :: env2) ->
+    EmptyEnv env1 /\ EmptyEnv env2.
+  Proof.
+    induction env1; intros.
+    - repeat constructor; assumption.
+    - simpl in *. destruct a.
+      + now apply EmptyEnv_app_cons in H.
+      + apply IHenv1 in H; destruct H.
+        repeat constructor; assumption.
+  Qed.
+
+  Lemma lookup_app_cons_weak : forall v env1 env2 T1 T2,
+    lookup v (None :: env1 ++ Some T1 :: env2) = Some T2 ->
+    lookup (v - 1) (env1 ++ Some T1 :: env2) = Some T2.
+  Proof.
+    induction v; intros; simpl in *.
+    - discriminate.
+    - now rewrite PeanoNat.Nat.sub_0_r.
+  Qed.
+
+  Lemma SingletonEnv_lookup_Some : forall env1 env2 T1 T2 v,
+    lookup v (env1 ++ Some T1 :: env2) = Some T2 ->
+    SingletonEnv (env1 ++ Some T1 :: env2) ->
+    T1 = T2.
+  Proof.
+    induction env1; intros.
+    - simpl in *.
+      destruct v.
+      + now inversion H.
+      + simpl in *.
+        apply EmptyEnv_lookup with (x := v) in H0.
+        rewrite H in H0; discriminate.
+    - simpl in *.
+      destruct a; simpl in *.
+      + now apply EmptyEnv_app_cons in H0.
+      + eapply IHenv1 with (v := v - 1) (env2 := env2).
+        * now apply lookup_app_cons_weak.
+        * assumption.
+  Qed.
+
+  From MailboxTypes Require Import Dblib.Environments.
+
+  Inductive EnvironmentSubtype' : Env -> Env -> Prop :=
+    | EnvSubtypeUn : forall env1 env2 x T,
+        lookup x env2 = None ->
+        Unrestricted T ->
+        EnvironmentSubtype' env1 env2 ->
+        EnvironmentSubtype' (insert x T env1) env2
+    | EnvSubtypeSub : forall env1 env2 x T1 T2,
+        Subtype T1 T2 ->
+        EnvironmentSubtype' env1 env2 ->
+        EnvironmentSubtype' (insert x T1 env1) (insert x T2 env2)
+    | EnvSubtypeTrans : forall env1 env2 env3,
+        EnvironmentSubtype' env1 env2 ->
+        EnvironmentSubtype' env2 env3 ->
+        EnvironmentSubtype' env1 env3
+    | EnvSubtypeRefl : forall env, EnvironmentSubtype' env env.
+
+  Lemma EnvSubtypeUn'_inv_EmptyEnv :
+    forall x env T', Unrestricted T' -> EnvironmentSubtype' (insert x T' env) env.
+  Proof.
+    intros.
+    constructor.
+  Admitted.
+
+  Lemma weakening : forall p env t T,
+    WellTypedTerm p env t T ->
+    forall x T' env',
+    Unrestricted T' ->
+    insert x T' env = env' ->
+    WellTypedTerm p env' (shift x t) T.
+  Proof.
+  Admitted.
+
+  Lemma subst_lemma_TValue : forall p env1 env2 env A A' B v1 v2 x,
+    WellTypedTerm p (insert x A env1) (TValue v1) B ->
+    WellTypedTerm p env2 (TValue v2) A' ->
+    A' ≤ A ->
+    env1 +ₑ env2 ~= env ->
+    WellTypedTerm p env (subst v2 x (TValue v1)) B.
+  Proof.
+    intros * WT1.
+    remember (insert x A env1) as E.
+    remember (TValue v1) as V.
+    revert x v1 v2 A A' env1 HeqE HeqV.
+    induction WT1; intros * ? ? WT2 Sub Dis; try discriminate.
+    - subst. simpl_subst_goal. simpl.
+      unfold subst_idx.
+      dblib_by_cases.
+      + admit.
+      + rewrite lift_zero. admit. (* this works with a few lemmas *)
+      + simpl. admit.
+    - subst. admit. (* EmptyEnv (insert x A env1) -> False *)
+    - subst. admit. (* EmptyEnv (insert x A env1) -> False *)
+    - subst. admit. (* EmptyEnv (insert x A env1) -> False *)
+    - subst. eapply SUB.
+      + apply EnvironmentSubtype_refl.
+      + eassumption.
+      + eapply IHWT1.
+
+
+  Lemma subst_lemma_TValue : forall p env1_1 env1_2 env2 env A A' B v1 v2,
+    WellTypedTerm p (env1_1 ++ Some A :: env1_2) (TValue v1) B ->
+    WellTypedTerm p env2 (TValue v2) A' ->
+    A' ≤ A ->
+    (env1_1 ++ None :: env1_2) +ₑ env2 ~= env ->
+    WellTypedTerm p env (subst v2 (length env1_1) (TValue v1)) B.
+  Proof.
+    intros * WT1.
+    remember (TValue v1) as V.
+    remember (env1_1 ++ Some A :: env1_2) as E.
+    revert env1_1 env1_2 v1 A HeqV HeqE v2 A' env2 env.
+    induction WT1; intros * Eq1 Eq2 * WT2 Sub Dis; try discriminate.
+    - injection Eq1; intros; subst.
+      simpl_subst_goal. simpl.
+      rewrite lift_zero.
+      Search (subst_idx).
+      assert (Greater : v > (length env1_1)). admit.
+      simpl_subst_goal.
+      (*rewrite subst_idx_miss_2.*)
+      (*+ simpl.*)
+      (*  generalize (SingletonEnv_lookup_Some _ _ _ _ _ H0 H).*)
+      (*  intros ->.*)
+      (*  constructor.*)
+      (**)
+      admit.
+    - subst; now apply EmptyEnv_app_cons in H.
+    - subst; now apply EmptyEnv_app_cons in H.
+    - subst; now apply EmptyEnv_app_cons in H.
+    - subst. induction env1_1.
+      + simpl in *.
+        simpl_subst_goal; simpl.
+        Search (lift _ 0 _).
+      
+      injection Eq1; intros ->; subst.
+
+(**
     We follow the method of Stark's Thesis 'Mechanising Syntax with Binders
     in Coq'.
 
@@ -161,60 +535,122 @@ Section subs_def.
     - repeat rewrite lift_Value_id; now rewrite IHt.
   Qed.
 
+  Lemma In_Some_EmptyEnv : forall env x, In (Some x) env -> ~ EmptyEnv env.
+  Proof.
+    intros * In; induction env.
+    - inversion In.
+    - destruct a; simpl in *; intros Empty.
+      + inversion Empty; subst; discriminate.
+      + destruct In.
+        * discriminate.
+        * inversion Empty; subst; now apply IHenv.
+  Qed.
+
+  Lemma subst_lemma_TValue : forall p env1 env2 env A A' B v1 v2,
+    (*lookup x env1 = (Some A) ->*)
+    WellTypedTerm p (Some A :: env1) (TValue v1) B ->
+    WellTypedTerm p env2 (TValue v2) A' ->
+    A' ≤ A ->
+    env1 +ₑ env2 ~= env ->
+    WellTypedTerm p env (subst_1 (TValue v1) v2) B.
+  Proof.
+
+
+  Lemma subst_lemma_TValue : forall p env1 env2 env A A' B v1 v2,
+    (*lookup x env1 = (Some A) ->*)
+    WellTypedTerm p (Some A :: env1) (TValue v1) B ->
+    WellTypedTerm p env2 (TValue v2) A' ->
+    A' ≤ A ->
+    env1 +ₑ env2 ~= env ->
+    WellTypedTerm p env (subst_1 (TValue v1) v2) B.
+  Proof.
+    intros * WT1.
+    remember (TValue v1) as V.
+    remember (Some A :: env1) as E.
+    revert HeqV HeqE v2 A' env2 env.
+    induction WT1; intros Eq1 Eq2 * WT2 Sub Dis; try discriminate.
+    + simpl. admit.
+    + subst. simpl. inversion H; subst. discriminate.
+    + subst. simpl. inversion H; subst. discriminate.
+    + subst. simpl. inversion H; subst. discriminate.
+    + subst.
+      inversion H; subst.
+      * admit.
+      * 
+      eapply SUB.
+      * apply EnvSubtypeRefl.
+      * apply H0.
+      * eapply IHWT1.
+        -- reflexivity.
+        -- admit.
+        -- apply WT2.
+        -- apply Sub.
+        -- 
+
+    destruct v1.
+    + inversion
+
   Lemma sub_lemma : forall p env1 env2 env A A' B v t,
+    (*In (Some A) env1 ->*)
     WellTypedTerm p (Some A :: env1) t B ->
     WellTypedTerm p env2 (TValue v) A' ->
     A' ≤ A ->
-    (None :: env1) +ₑ env2 ~= env ->
-    WellTypedTerm p env (t[v..]) B.
+    env1 +ₑ env2 ~= env ->
+    WellTypedTerm p env (subst_1 t v) B.
   Proof.
-    (*intros * WT1 WT2 Sub Dis.*)
-    (*remember (Some A :: env1) as env1' eqn:E.*)
-    (*generalize dependent env1.*)
-    (*induction WT1 using @WellTypedTerm_ind3 with*)
-    (*  (P0 := fun _ _ _ _ => True)*)
-    (*  (P1 := fun _ _ _ _ => True).*)
-    (*intros * WT1.*)
-    (*revert env2 env v A'.*)
-    (*remember (Some A :: env1) as env1' eqn:E.*)
-    (*generalize dependent A.*)
-    (*generalize dependent env1.*)
-    (*induction WT1; intros.*)
-    (*- simpl in *.*)
-    (*  assert (zero : v = 0). admit.*)
-    (*  assert (SubTy : T = A). admit.*)
-    (*  subst. simpl.*)
-    (*  (*rewrite subst_1_Var_0.*)*)
-    (*  eapply SUB with (env2 := env2).*)
-    (*  (* env1 is empty, thus env2 = env *)*)
-    (*  admit.*)
-    (*  apply H2.*)
-    (*  apply H1.*)
-    (*- inversion H; subst; discriminate.*)
-    (*- inversion H; subst; discriminate.*)
-    (*- inversion H; subst; discriminate.*)
-    (*- eapply APP.*)
-    (*  + apply H.*)
-    (*  + eapply IHWT1. apply E. apply H0. assumption. assumption.*)
-    (*- subst.*)
-    (*  inversion H; subst.*)
-    (*  + eapply LET.*)
-    (*    * apply (EnvironmentDis_implies_Comb _ _ _ H2).*)
-    (*    * eapply IHWT1_1.*)
-    (*      -- reflexivity.*)
-    (*      -- apply H0.*)
-    (*      -- assumption.*)
-    (*      -- admit.*)
-    (*- admit.*)
-    (*- subst; inversion H; subst; discriminate.*)
-    (*- admit.*)
-    (*- admit.*)
-    (*- subst. inversion H3; subst; inversion H; subst.*)
-    (*  + eapply SUB.*)
-    (*    * apply EnvSubtypeRefl.*)
-    (*    * apply H0.*)
-    (*    * eapply IHWT1.*)
-    (*      -- *)
+    intros * In WT1.
+    (*remember env1 as env1' eqn: E.*)
+    revert In.
+    induction WT1 using @WellTypedTerm_ind3 with
+      (P0 := fun _ _ _ _ => True)
+      (P1 := fun _ _ _ _ => True).
+    - intros In WT2 Sub Dis.
+      simpl. admit.
+    - intros. admit. (* not possible *)
+    - intros. admit. (* not possible *)
+    - intros. admit. (* not possible *)
+    - intros. simpl.
+
+    revert env2 env v A'.
+    remember (Some A :: env1) as env1' eqn:E.
+    generalize dependent A.
+    generalize dependent env1.
+    induction WT1; intros.
+    - simpl in *.
+      assert (zero : v = 0). admit.
+      assert (SubTy : T = A). admit.
+      subst. simpl.
+      (*rewrite subst_1_Var_0.*)
+      eapply SUB with (env2 := env2).
+      (* env1 is empty, thus env2 = env *)
+      admit.
+      apply H2.
+      apply H1.
+    - inversion H; subst; discriminate.
+    - inversion H; subst; discriminate.
+    - inversion H; subst; discriminate.
+    - eapply APP.
+      + apply H.
+      + eapply IHWT1. apply E. apply H0. assumption. assumption.
+    - subst.
+      inversion H; subst.
+      + eapply LET.
+        * apply (EnvironmentDis_implies_Comb _ _ _ H2).
+        * eapply IHWT1_1.
+          -- reflexivity.
+          -- apply H0.
+          -- assumption.
+          -- admit.
+    - admit.
+    - subst; inversion H; subst; discriminate.
+    - admit.
+    - admit.
+    - subst. inversion H3; subst; inversion H; subst.
+      + eapply SUB.
+        * apply EnvSubtypeRefl.
+        * apply H0.
+        * eapply IHWT1.
+          -- 
     Admitted.
 
 End subs_def.
