theories/MailboxCalculus.v
@@ -1,0 +1,137 @@
+(** * Syntax of the Mailbox Calculus *)
+
+From MailboxTypes Require Import Types.
+From MailboxTypes Require Import Message.
+From MailboxTypes Require Import Util.
+
+From Stdlib Require Import Lists.List.
+Import ListNotations.
+From Stdlib Require Import Compare_dec.
+
+Generalizable All Variables.
+
+Section definition_def.
+
+(** We define a set of definition names to avoid dealing with
+    function names. We assume they are defined before the
+    program is executed.
+*)
+Class IDefinitionName DefinitionName : Type :=
+  {
+    eq_dec : forall m n, {@eq DefinitionName m n} + {~ @eq DefinitionName m n}
+  }.
+
+End definition_def.
+
+Section syntax_def.
+
+Context `{M : IMessage Message}.
+Context `{D : IDefinitionName DefinitionName}.
+
+Inductive Fin : nat -> Type :=
+  | z : forall n, Fin (S n)
+  | s : forall n, Fin n -> Fin (S n).
+
+(** A variable is just a natural number bounded by some number n *)
+Definition Name n := Fin n.
+
+(** We associated values as relations between environments and types.
+    Since variables are treated as values, we need a way to check what
+    their type is.
+*)
+(*Inductive Value : Type :=*)
+(*    ValueBool : bool -> Value*)
+(*  | ValueUnit : Value*)
+(*  | ValueVar  : Name -> Value.*)
+
+Type pred.
+
+(** Terms of the language *)
+Inductive Process `{IMessage Message} `{IDefinitionName DefinitionName} (n : nat) : Type :=
+  | PDone : Process n
+  | PInv : DefinitionName -> Name n -> Process n
+  | PGuard : Guard n -> Process n
+  | PSend : Name n -> Message -> Name n -> Process n
+  | PPar : Process n -> Process n -> Process n
+  | PRes : Process (S n) -> Process n
+  with Guard `{IMessage Message} `{IDefinitionName DefinitionName} (n : nat) : Type :=
+  | GFail : Name n -> Guard n
+  | GFree : Name n -> Process (pred n) -> Guard n
+  | GReceive : Name n -> Message -> Name n -> Process (S n) -> Guard n
+  | GComp : Guard n -> Guard n -> Guard n.
+
+Arguments PDone {_} {_} {_}.
+
+(** Function definitions *)
+Inductive FunctionDefinition : Type :=
+  | FunDef : DefinitionName ->  (* Function name *)
+             TUsage ->          (* Argument type *)
+             TUsage ->          (* Result type *)
+             Process 1 ->            (* Function body *)
+             FunctionDefinition.
+
+(** A program is a collection of definitions, an initial term and a
+    mapping from message to the content's type
+*)
+Record Prog : Type :=
+  {
+    signature : Message -> TType
+  ; definitions : DefinitionName -> FunctionDefinition
+  ; initialTerm : Process 0
+  }.
+
+(** Defining the mutual recursion scheme for [Process] *)
+Scheme Process_ind2 := Induction for Process Sort Prop
+  with Guard_ind2 := Induction for Guard Sort Prop.
+
+End syntax_def.
+
+Declare Scope process_scope.
+Notation "'done'" := (PDone _) (at level 1).
+Notation "X [ v ]" := (PInv _ X v) (at level 7, format "X '/' [ v ]").
+(* TODO: Guard *)
+Notation "u '!' '<' m '>[' v ']'" := (PSend _ u m v) (at level 7, format "u '/' ! '/' < m '/' >[ v ]").
+Notation "A ∥ B" := (PPar _ A B) (at level 10).
+Notation "'𝝂' P" := (PRes _ P) (at level 9).
+Notation "'fail' u" := (GFail _ u) (at level 1).
+Notation "'free' u ';' P" := (GFree _ u P) (at level 7).
+Notation "u ? m ';' P" := (GReceive _ u m P) (at level 7).
+Notation "G '|+|' H" := (GComp _ G H) (at level 10, left associativity).
+
+Section Examples.
+
+Context `{M : IMessage Message}.
+Context `{D : IDefinitionName DefinitionName}.
+
+Definition TestProcess : Process 0 := 𝝂 done.
+
+(** [Future] defines the message atoms *)
+Inductive Data : Type := data : Data.
+
+(** We show that [Future] has decidable equality *)
+Instance DataMessage : IMessage Data.
+Proof.
+  constructor.
+  - destruct m; destruct n;
+    try (now left);
+    try (now right).
+  - apply (fun _ => 1).
+Defined.
+
+Definition ExampleProcess : Process 0.
+Proof.
+  apply PRes.
+  apply PRes.
+  apply PRes.
+  apply PGuard.
+  apply GComp.
+  + apply GFree. apply z. apply PDone.
+  + apply GComp.
+    apply GFree. apply z. apply PDone.
+    apply GFree. apply z. apply PDone.
+Defined.
+
+Print ExampleProcess.
+
+End Examples.
+
